backend/Mach.v
@@ -420,7 +420,7 @@ Inductive step: state -> trace -> state -> Prop :=
       let sp := Vptr stk Ptrofs.zero in
       store_stack m1 sp Tptr f.(fn_link_ofs) (parent_sp s) = Some m2 ->
       store_stack m2 sp Tptr f.(fn_retaddr_ofs) (parent_ra s) = Some m3 ->
-      Mem.record_stack_blocks m3 (Some (frame_with_info stk (Some (fn_frame f)))) (fn_stacksize f) = Some m1_ ->
+      Mem.record_stack_blocks m3 (stk::nil, Some (fn_frame f),fn_stacksize f) m1_ ->
       rs' = undef_regs destroyed_at_function_entry rs ->
       step (Callstate s fb rs m)
         E0 (State s fb sp f.(fn_code) rs' m1_)
