common/Memimpl.v
@@ -6157,23 +6157,6 @@ Proof.
   rewrite Zplus_0_r in H1; auto.
 Qed.
 
-Lemma stack_inject_nil:
-  forall f p,
-    stack_inject f (fun _ => None) p nil nil.
-Proof.
-  constructor.
-  - red. congruence.
-  - congruence.
-  - intros b1 b2 delta FB i1 f1 FAP IFR.
-    inv FAP. simpl in H. rewrite nth_error_nil in H; congruence.
-  - simpl. congruence.
-  - congruence.
-  - simpl; intros; omega.
-  - simpl; intros; omega.
-  - congruence.
-  - congruence.
-Qed.
-
 Theorem empty_inject_neutral:
   forall thr, inject_neutral thr empty.
 Proof.
